\begin{lemma}{Gaussian Hypergeometric Function}{gaussian-hypergeometric-function}
  The $p=2$, $q=1$ special case of the generalised hypergeometric series, commonly referred to as the Gaussian hypergeometric function, can also be evaluated by
  $${}_2F_1\left(\begin{matrix}a_{1}, -n \\b_{1}\end{matrix}; z\right) = \sum_{k=0}^n (-1)^k \binom{n}{k} \frac{(a_1)_k}{(b_1)_k}z^k\,,$$
  when the second argument $a_2 = -n$ is a nonpositive integer, so $n \in \N_0$.
\end{lemma}
\begin{proof}
  Starting from the definition of the generalised hypergeometric series ${}_pF_q$ with $p=2$ and $q=1$ (\Cref{def:generalised-hypergeometric-series}),
  $${}_2F_1\left(\begin{matrix}a_{1}, -n \\b_{1}\end{matrix}; z\right) = \sum_{k=0}^{\infty} \frac{(a_1)_k (-n)_k}{(b_1)_k} \frac{z^k}{k!} = \sum_{k=0}^{n} \frac{(a_1)_k (-n)_k}{(b_1)_k} \frac{z^k}{k!}\,,$$
  which can be terminated at $k=n$ due to \Cref{remark:nonpositive-pochhammer}, we can express
  $$\frac{(-n)_k}{k!} = \binom{-n+k-1}{k} = (-1)^k \binom{1+n-k+k-1}{k} = (-1)^k \binom{n}{k}$$
  using a well-known relation between the Pochhammer symbol and the binomial coefficient which immediately leads us to
  $${}_2F_1\left(\begin{matrix}a_{1}, -n \\b_{1}\end{matrix}; z\right) = \sum_{k=0}^n \binom{n}{k} \frac{(a_1)_k}{(b_1)_k}(-z)^k\,,$$
  concluding the proof.
\end{proof}

Note that these functions are generally tricky to evaluate efficiently, recent advancements have enabled their usage in a broader range of applications \parencite{2008-hypergeometric-functions-jl-1,2017-hypergeometric-functions-jl-2,2023-hypergeometric-functions-jl-3}.
Implementations are available in the \href{https://github.com/JuliaMath/HypergeometricFunctions.jl}{HypergeometricFunctions.jl} package in Julia.
